raft-proofs/VotesVotesWithLogCorrespondProof.v
@@ -28,7 +28,72 @@ Section VotesVotesWithLogCorrespond.
       | [ H : context [ update _ ?y _ ?x ] |- _ ] => destruct (name_eq_dec y x)
     end.
 
+  Lemma votes_votesWithLog_correspond_cases :
+    forall net h gd d ps' st',
+      votes_votesWithLog_correspond net ->
+      (forall h' : Net.name, st' h' = update (nwState net) h (gd, d) h') ->
+      (votes gd = votes (fst (nwState net h)) /\  (* unchanged *)
+       votesWithLog gd = votesWithLog (fst (nwState net h))) \/
+      (exists t n l,  (* add entry *)
+       votes gd = (t, n) :: votes (fst (nwState net h)) /\
+       votesWithLog gd = (t, n, l) :: votesWithLog (fst (nwState net h))) ->
+      votes_votesWithLog_correspond {| nwPackets := ps'; nwState := st' |}.
+  Proof.
+    red. unfold votes_votesWithLog_correspond. split; intros; break_and.
+    - unfold votes_votesWithLog in *; intros.
+      repeat find_higher_order_rewrite; update_destruct; rewrite_update; [|eauto].
+      simpl in *. break_or_hyp; repeat break_exists; break_and.
+      + repeat find_rewrite. eauto.
+      + repeat find_rewrite. simpl in *. intuition; try tuple_inversion; eauto.
+    - unfold votesWithLog_votes in *; intros.
+      repeat find_higher_order_rewrite; update_destruct; rewrite_update; [|eauto].
+      simpl in *. break_or_hyp; repeat break_exists; break_and.
+      + repeat find_rewrite. eauto.
+      + repeat find_rewrite. simpl in *. intuition.
+        * eexists. tuple_inversion. intuition.
+        * find_apply_hyp_hyp. break_exists. eexists. eauto.
+  Qed.
+
+  Ltac start :=
+    red; intros; eapply votes_votesWithLog_correspond_cases; eauto.
+
+  Ltac finish :=
+    repeat break_match; subst_max; first [
+      left; solve[eauto] |
+      right; repeat eexists; solve[eauto]
+    ].
+
+  Ltac unfold_all :=
+    red; unfold votes_votesWithLog_correspond, votes_votesWithLog, votesWithLog_votes.
+
+  Lemma votes_votesWithLog_correspond_invariant :
+    forall net,
+      refined_raft_intermediate_reachable net ->
+      votes_votesWithLog_correspond net.
+  Proof.
+    intros.
+    apply refined_raft_net_invariant; auto.
+    - unfold_all. simpl. split; contradiction.
+    - start. unfold update_elections_data_client_request in *. finish.
+    - start. unfold update_elections_data_timeout in *. finish.
+    - start. unfold update_elections_data_appendEntries in *. finish.
+    - start. subst; auto.
+    - start. unfold update_elections_data_requestVote in *. finish.
+    - start. unfold update_elections_data_requestVoteReply in *. finish.
+    - start. find_rewrite. auto.
+    - start. find_rewrite. auto.
+    - unfold_all. split; intros; break_and;
+      repeat find_reverse_higher_order_rewrite; eauto.
+    - unfold_all. split; intros; break_and.
+      + find_higher_order_rewrite. update_destruct; subst; rewrite_update; [|eauto].
+        unfold reboot in *. simpl in *. specialize (H1 h0). repeat find_rewrite. simpl in *. eauto.
+      + find_higher_order_rewrite. update_destruct; subst; rewrite_update; [|eauto].
+        unfold reboot in *. simpl in *. specialize (H7 h0). repeat find_rewrite. simpl in *. eauto.
+  Qed.
+
   Instance vvci : votes_votesWithLog_correspond_interface.
   Proof.
-  Admitted.
+    split. exact votes_votesWithLog_correspond_invariant.
+  Defined.
+
 End VotesVotesWithLogCorrespond.
